src/go_lang/interpreter/tests.v
@@ -1,0 +1,86 @@
+From Perennial.go_lang Require Import prelude.
+From Perennial.go_lang.interpreter Require Import interpret_types.
+From Perennial.go_lang.interpreter Require Import interpreter.
+From Perennial.go_lang.interpreter Require Import disk_interpreter.
+
+From Perennial.go_lang.examples Require Import goose_unittest.
+From Perennial.go_lang.ffi Require Import disk.
+Require Import Program.
+
+Definition startstate : state := inhabitant.
+
+Definition testRec : expr :=
+  (rec: BAnon BAnon :=
+     #3 + #3).
+
+Definition testLiteralCast: expr :=
+  λ: <>,
+     let: "x" := #2 in
+     (Var "x") + #2.
+
+Definition testIfStatement: expr :=
+  λ: <>,
+     let: "m" := #2 in
+     (if: (Var "m") > #3
+      then #3
+      else #1).
+
+Definition testMatch: val :=
+  λ: "x",
+  match: (Var "x") with
+    InjL "x1" => #3 + (Var "x1")
+  | InjR "x1" => #4 + (Var "x1")
+  end.
+
+Compute (runStateT (interpret 10 (AllocN #1 (zero_val uint32T))) startstate).
+Compute (runStateT (interpret 10 (returnTwoWrapper #3)) startstate).
+Compute (runStateT (interpret 10 (testRec #0)) startstate).
+
+Definition run (p: expr): Error val :=
+  fst <$> runStateT (interpret 100 p) startstate.
+
+Notation check_run p := (ltac:(let x := (eval vm_compute in (run p)) in
+                               lazymatch x with
+                               | Works _ ?v => exact v
+                               | Fail _ ?msg => fail "interpreter failed on" p msg
+                               end)) (only parsing).
+
+Definition runs_to (p: expr) (v: val) :=
+  run p = Works _ v.
+Notation "p ~~> v" := (eq_refl : runs_to p v) (at level 70).
+
+Example run_testRec := testRec #0 ~~> #6.
+
+Compute (check_run (testIfStatement #())).
+Compute (check_run (testMatch (InjL #2))).
+Compute (check_run (testMatch (InjR #2))).
+Compute (check_run (testLiteralCast #())).
+
+(* Functions from examples/goose_unittests *)
+Compute (check_run ConstWithArith).
+Compute (check_run (useMap #())).
+Compute (check_run (useSliceIndexing #())).
+Compute (check_run (ReassignVars #())).
+
+Definition test_case (p: expr) :=
+  match (fst <$> runStateT (interpret 100 p) startstate) with
+  | Works _ (LitV (LitBool true)) => true
+  | _ => false
+  end.
+
+(* fails because #333 is a uint64 *)
+Fail Compute (check_run (EncDec32 #333)).
+Definition tc1 := (test_case (EncDec64 #333)).
+Definition tc2 := (test_case (EncDec32 #(U32 333))).
+Example tc1_ok : tc1 = true := eq_refl.
+Example tc2_ok : tc2 = true := eq_refl.
+
+(* Extraction testing:
+
+Require Coq.extraction.Extraction.
+Extraction Language Haskell.
+Extract Inductive bool => "GHC.Base.Bool" [ "GHC.Base.True" "GHC.Base.False" ].
+
+Extraction "tc1.hs" tc1.
+
+*)
